src/Language/PlutusIR/Semantics/Static/Theorems/FreeInContext.v
@@ -1,5 +1,8 @@
 Require Import PlutusCert.Language.PlutusIR.
+Require Import PlutusCert.Util.List.
 Import NamedTerm.
+Require Import Lists.List.
+Import ListNotations.
 
 Require Import PlutusCert.Language.PlutusIR.Semantics.Static.Theorems.ContextInvariance.AFI.
 Require Import PlutusCert.Language.PlutusIR.Semantics.Static.Theorems.In_Auxiliary.
@@ -11,21 +14,21 @@ Module Ty.
     Delta |-* T : K ->
     forall X,
       Ty.appears_free_in X T ->
-      exists K', Delta X = Datatypes.Some K'.
+      exists K', lookup X Delta = Datatypes.Some K'.
   Proof with eauto.
     induction 1.
     all: intros X0 Hafi.
     all: try solve [inversion Hafi; subst; eauto].
     - inversion Hafi. subst.
       eapply IHhas_kind in H5.
-      rewrite update_neq in H5...
+      rewrite lookup_neq in H5...
     - inversion Hafi. subst.
       eapply IHhas_kind in H5.
-      rewrite update_neq in H5...
+      rewrite lookup_neq in H5...
   Qed.
 
   Corollary kindable_empty__closed : forall T K,
-      empty |-* T : K ->
+      [] |-* T : K ->
       Ty.closed T.
   Proof with eauto.
     intros. unfold Ty.closed.
@@ -39,28 +42,28 @@ End Ty.
 
 Module Term.
 
-  Definition P_has_type (Delta : Delta) (Gamma : Gamma) (t : Term) (T : Ty) :=
+  Definition P_has_type (Delta : list (string * Kind)) (Gamma : list (string * Ty)) (t : Term) (T : Ty) :=
     forall x,
       Term.appears_free_in x t ->
-      exists T', Gamma x = Datatypes.Some T'.
+      exists T', lookup x Gamma = Datatypes.Some T'.
       
-  Definition P_constructor_well_formed (Delta : Delta) (c : constructor) (T : Ty) :=
+  Definition P_constructor_well_formed (Delta : list (string * Kind)) (c : constructor) (T : Ty) :=
     Delta |-ok_c c : T.
 
-  Definition P_bindings_well_formed_nonrec (Delta : Delta) (Gamma : Gamma) (bs : list Binding) :=
+  Definition P_bindings_well_formed_nonrec (Delta : list (string * Kind)) (Gamma : list (string * Ty)) (bs : list Binding) :=
     forall x,
       Term.appears_free_in__bindings_nonrec x bs ->
-      exists T', Gamma x = Datatypes.Some T'.
+      exists T', lookup x Gamma = Datatypes.Some T'.
 
-  Definition P_bindings_well_formed_rec  (Delta : Delta) (Gamma : Gamma) (bs : list Binding) :=
+  Definition P_bindings_well_formed_rec  (Delta : list (string * Kind)) (Gamma : list (string * Ty)) (bs : list Binding) :=
     forall x,
       Term.appears_free_in__bindings_rec x bs ->
-      exists T', Gamma x = Datatypes.Some T'.
+      exists T', lookup x Gamma = Datatypes.Some T'.
 
-  Definition P_binding_well_formed (Delta : Delta) (Gamma : Gamma) (b : Binding) :=
+  Definition P_binding_well_formed (Delta : list (string * Kind)) (Gamma : list (string * Ty)) (b : Binding) :=
     forall x,
       Term.appears_free_in__binding x b ->
-      exists T', Gamma x = Datatypes.Some T'.
+      exists T', lookup x Gamma = Datatypes.Some T'.
 
   #[export] Hint Unfold
     P_has_type
@@ -89,14 +92,14 @@ Module Term.
     - (* T_LamAbs *)
       inversion Hafi. subst.
       eapply H2 in H8...
-      rewrite update_neq in H8...
+      rewrite lookup_neq in H8...
     - (* T_Let *)
       inversion Hafi.
       + subst.
         eapply H5 in H12...
         apply notIn_bvbs_bindsG in H10.
         eapply notIn__map_normalise in H10...
-        rewrite notIn__lookup_mupdate in H12...
+        rewrite notIn__lookup_append in H12...
       + subst.
         eapply H3 in H9...
     - (* T_LetRec *)
@@ -105,12 +108,12 @@ Module Term.
         eapply H5 in H12...
         apply notIn_bvbs_bindsG in H10.
         eapply notIn__map_normalise in H10...
-        rewrite notIn__lookup_mupdate in H12...
+        rewrite notIn__lookup_append in H12...
       + subst.
         eapply H3 in H11...
         apply notIn_bvbs_bindsG in H10.
         eapply notIn__map_normalise in H10...
-        rewrite notIn__lookup_mupdate in H11...
+        rewrite notIn__lookup_append in H11...
     - (* W_ConsB_NonRec *)
       inversion Hafi. 
       + subst.
@@ -118,37 +121,37 @@ Module Term.
       + subst.
         apply notIn_bvb_bindsG in H7.
         eapply notIn__map_normalise in H7...
-        erewrite <- notIn__lookup_mupdate...
+        erewrite <- notIn__lookup_append...
 Qed.
 
 End Term.
 
 Module Annotation.
 
-  Definition P_has_type (Delta : Delta) (Gamma : Gamma) (t : Term) (T : Ty) :=
+  Definition P_has_type (Delta : list (string * Kind)) (Gamma : list (string * Ty)) (t : Term) (T : Ty) :=
     forall X,
       Annotation.appears_free_in X t ->
-      exists K', Delta X = Datatypes.Some K'.
+      exists K', lookup X Delta = Datatypes.Some K'.
       
-  Definition P_constructor_well_formed (Delta : Delta) (c : constructor) (T : Ty) :=
+  Definition P_constructor_well_formed (Delta : list (string * Kind)) (c : constructor) (T : Ty) :=
     forall X,
       Annotation.appears_free_in__constructor X c ->
-      exists K', Delta X = Datatypes.Some K'.
+      exists K', lookup X Delta = Datatypes.Some K'.
 
-  Definition P_bindings_well_formed_nonrec (Delta : Delta) (Gamma : Gamma) (bs : list Binding) :=
+  Definition P_bindings_well_formed_nonrec (Delta : list (string * Kind)) (Gamma : list (string * Ty)) (bs : list Binding) :=
     forall X,
       Annotation.appears_free_in__bindings_nonrec X bs ->
-      exists K', Delta X = Datatypes.Some K'.
+      exists K', lookup X Delta = Datatypes.Some K'.
 
-  Definition P_bindings_well_formed_rec (Delta : Delta) (Gamma : Gamma) (bs : list Binding) :=
+  Definition P_bindings_well_formed_rec (Delta : list (string * Kind)) (Gamma : list (string * Ty)) (bs : list Binding) :=
     forall X,
       Annotation.appears_free_in__bindings_rec X bs ->
-      exists K', Delta X = Datatypes.Some K'.
+      exists K', lookup X Delta = Datatypes.Some K'.
 
-  Definition P_binding_well_formed (Delta : Delta) (Gamma : Gamma) (b : Binding) :=
+  Definition P_binding_well_formed (Delta : list (string * Kind)) (Gamma : list (string * Ty)) (b : Binding) :=
     forall X,
       Annotation.appears_free_in__binding X b ->
-      exists K', Delta X = Datatypes.Some K'.
+      exists K', lookup X Delta = Datatypes.Some K'.
 
     
   #[export] Hint Unfold
@@ -178,13 +181,13 @@ Module Annotation.
       inversion Hafi.
       subst.
       eapply H0 in H5...
-      rewrite update_neq in H5...
+      rewrite lookup_neq in H5...
     - (* T_Let*)
       inversion Hafi.
       + subst.
         eapply H5 in H11...
         apply notIn_btvbs_bindsD in H9.
-        rewrite notIn__lookup_mupdate in H11...
+        rewrite notIn__lookup_append in H11...
       + subst.
         eapply H3 in H8...
     - (* T_LetRec *)
@@ -192,11 +195,11 @@ Module Annotation.
       + subst.
         eapply H5 in H11...
         apply notIn_btvbs_bindsD in H9.
-        rewrite notIn__lookup_mupdate in H11...
+        rewrite notIn__lookup_append in H11...
       + subst.
         eapply H3 in H10...
         apply notIn_btvbs_bindsD in H9.
-        rewrite notIn__lookup_mupdate in H10...
+        rewrite notIn__lookup_append in H10...
     - (* W_Con *)
       inversion Hafi. subst.
       rewrite <- H3 in H.
@@ -209,18 +212,18 @@ Module Annotation.
         apply H0...
       + subst.
         apply notIn_btvb_bindsD in H6.
-        erewrite <- notIn__lookup_mupdate...
+        erewrite <- notIn__lookup_append...
     - (* W_Data *)
       inversion Hafi. subst.
       destruct H7 as [c [HIn__c Hafi__c]].
-      erewrite <- notIn__lookup_mupdate...
+      erewrite <- notIn__lookup_append...
       eapply H1...
   Qed.
 
 End Annotation.
 
 Corollary typable_empty__closed : forall t T,
-    empty ,, empty |-+ t : T ->
+    [] ,, [] |-+ t : T ->
     closed t.
 Proof with eauto.
   intros. unfold closed.
