src/Util/List.v
@@ -2,15 +2,210 @@ Require Import Coq.Lists.List.
 Require Import Coq.Strings.String.
 Import ListNotations.
 
-Local Open Scope list_scope.
 Local Open Scope string_scope.
-
-
+Local Open Scope list_scope.
+Import ListNotations.
 Fixpoint lookup {X:Type} (k : string) (l : list (string * X)) : option X :=
   match l with
   | nil => None
   | (j,x) :: l' => if j =? k then Datatypes.Some x else lookup k l'
   end.
+
+Lemma lookup_eq {X} k (v : X) kvs : lookup k ((k, v) :: kvs) = Some v.
+Proof.
+  simpl.
+  destruct (k =? k) eqn:H_eqb.
+  - reflexivity.
+  - rewrite eqb_neq in H_eqb.
+    contradiction.
+Qed.
+
+Lemma lookup_neq {X} k1 k2 (v : X) kvs : k1 <> k2 -> lookup k1 ((k2, v) :: kvs) = lookup k1 kvs.
+Proof with auto.
+  intros H_neq.
+  simpl.
+  rewrite eqb_sym.
+  rewrite <- eqb_neq in H_neq.
+  rewrite H_neq...
+Qed.
+
+Lemma In__lookup_append {X : Type} k (kvs : list (string * X)) ys zs :
+  In k (map fst kvs) ->
+  lookup k (kvs ++ ys) = lookup k (kvs ++ zs).
+Proof.
+  intros H_In.
+  induction kvs.
+  - inversion H_In.
+  - destruct a.
+    destruct (string_dec k s); subst.
+    + simpl.
+      assert (H : s =? s = true). { rewrite eqb_eq. reflexivity. }
+      rewrite H.
+      reflexivity.
+    + simpl.
+      assert (H : s =? k = false). { rewrite -> eqb_sym. rewrite eqb_neq. assumption. }
+      rewrite H.
+      destruct H_In.
+        * destruct H0. contradiction.
+        * auto.
+Qed.
+
+Lemma notIn__lookup_append {X : Type} k (kvs : list (string * X)) ys :
+     ~ In k (map fst ys) -> lookup k (ys ++ kvs) = lookup k kvs.
+Proof with auto.
+  intros H_notIn.
+  induction ys...
+  destruct a.
+  simpl in H_notIn.
+  destruct (string_dec s k).
+  - assert (s = k \/ In k (map fst ys)) by auto.
+    contradiction.
+  - rewrite <- eqb_neq in n.
+    simpl.
+    rewrite n.
+    assert (~ In k (map fst ys))...
+Qed.
+
+Lemma lookup_append_cong {X : Type} k (new kvs kvs' : list (string * X)) :
+  lookup k kvs = lookup k kvs' -> 
+  lookup k (new ++ kvs) = lookup k (new ++ kvs').
+Proof with auto.
+  intros H_kvs_kvs'.
+  induction new...
+  - destruct a.
+    destruct (eqb s k) eqn:H_eqb.
+    all: simpl; rewrite H_eqb...
+Qed.
+
+Definition inclusion {A : Type} (m m' : list (string * A)) :=
+  forall x v, lookup x m = Some v -> lookup x m' = Some v.
+
+Lemma inclusion_tail {A : Type} (x : string * A) m m' :
+  inclusion m m' ->
+  inclusion (x :: m) (x :: m').
+Proof.
+  intro H_incl.
+  destruct x.
+  intros k v.
+  destruct (s =? k) eqn:H_eqb.
+  all: simpl; rewrite H_eqb; auto.
+Qed.
+
+Lemma inclusion_refl {A} (xs : list (string * A)) :
+  inclusion xs xs.
+Proof with auto.
+  unfold inclusion.
+  intros.
+  induction xs...
+Qed.
+
+Lemma inclusion_trans : forall A (m1 m2 m3 : list (string * A)), inclusion m1 m2 ->
+  inclusion m2 m3 -> inclusion m1 m3.
+Proof with auto.
+  unfold inclusion...
+Qed.
+
+Lemma inclusion_cons A (m m' : list (string * A)) x vx :
+  inclusion m m' -> inclusion ((x, vx) :: m) ((x, vx) :: m').
+Proof with auto.
+  intros H_incl.
+  unfold inclusion.
+  intros y vy H_lookup_y.
+  destruct (eqb x y) eqn:H_eqb.
+  all: simpl in *; rewrite H_eqb in *...
+Qed.
+
+Lemma inclusion_append {A} m m' (kvs : list (string * A)) :
+  inclusion m m' -> inclusion (kvs ++ m) (kvs ++ m').
+Proof with auto.
+  intros H_incl.
+  induction kvs...
+  unfold inclusion. intros.
+  destruct a.
+  destruct (eqb s x) eqn:H_eqb.
+  all: simpl in *;
+    rewrite H_eqb in *...
+Qed.
+
+Lemma cons_shadow {A} k (x y : A) xs:
+  inclusion ((k, x) :: (k, y) :: xs) ((k, x) :: xs).
+Proof with auto.
+  unfold inclusion.
+  intros l w H_lookup.
+  simpl in *.
+  destruct (k =? l) eqn:H_eqb...
+Qed.
+
+Lemma append_shadow {A} k (v : A) xs ys :
+  In k (map fst xs) -> inclusion (xs ++ ((k, v) :: ys)) (xs ++ ys).
+Proof.
+Admitted.
+
+Lemma cons_permute A (m : list (string * A)) x1 x2 v1 v2 :
+  x2 <> x1 -> inclusion ((x1, v1) :: (x2 , v2) :: m) ((x2, v2) :: (x1, v1) :: m).
+Proof with auto.
+  unfold inclusion.
+  intros H_neq x v.
+  destruct (x1 =? x) eqn:H_x_x1;
+  destruct (x2 =? x) eqn:H_x_x2.
+  all: try (simpl; rewrite H_x_x1, H_x_x2; auto).
+  assert (x2 = x1).
+    { rewrite -> eqb_eq in *.
+      apply eq_sym in H_x_x2. 
+      transitivity x...
+    }
+  contradiction.
+Qed.
+
+Lemma append_permute A (m : list (string * A)) k (v : A) xs ys:
+  ~ (In k (map fst xs)) -> inclusion (xs ++ ((k, v) :: ys)) ((k, v) :: xs ++ ys) .
+Admitted.
+
+Definition equivalent {A : Type} (m m' : list (string * A)) :=
+  inclusion m m' /\ inclusion m' m.
+
+Lemma equivalent_refl : forall A (m : list (string * A)), equivalent m m.
+Proof.
+  unfold equivalent.
+  auto using inclusion_refl.
+Qed.
+
+Lemma equivalent_sym : forall A (m m' : list (string * A)), equivalent m m' -> equivalent m' m.
+Proof.
+  unfold equivalent, inclusion.
+  intros.
+  easy.
+Qed.
+
+Lemma equivalent_trans : forall A (m1 m2 m3 : list (string * A)), equivalent m1 m2 ->
+  equivalent m2 m3 -> equivalent m1 m3.
+Proof.
+  unfold equivalent, inclusion.
+  intros.
+  destruct H, H0.
+  auto.
+Qed.
+
+Require Import Coq.Classes.RelationClasses.
+
+Global Instance inclusion_reflexive : forall (A : Type), Reflexive (@inclusion A) := @inclusion_refl.
+Global Instance inclusion_transitive : forall (A : Type), Transitive (@inclusion A) := inclusion_trans.
+
+Global Instance equivalent_reflexive : forall (A : Type), Reflexive (@equivalent A) := equivalent_refl.
+Global Instance equivalent_symmetric : forall (A : Type), Symmetric (@equivalent A) := equivalent_sym.
+Global Instance equivalent_transitive : forall (A : Type), Transitive (@equivalent A) := equivalent_trans.
+Global Instance equivalent_equivalence : forall (A : Type), Equivalence (@equivalent A) := { }.
+
+(*
+Add Parametric Relation (A : Type) : (list (string * A)) (equivalent)
+  reflexivity proved by (equivalent_refl A)
+  symmetry proved by (equivalent_sym A)
+  transitivity proved by (equivalent_trans A) as tests.
+
+Definition my_setoid : Setoid := _.
+Global Instance equivalent_Setoid : forall (A : Type), Setoid (@equivalent A) := _.
+*)
+
 
 Fixpoint lookup' {A X : Type} (A_eqb : A -> A -> bool) (k : A) (l : list (A * X)) : option X :=
   match l with
@@ -25,6 +220,14 @@ Inductive Lookup {A B :Type} (k : A) (v : B) : list (A * B) -> Prop :=
 
 Lemma Lookup_lookup : forall A k (v : A) kvs, Lookup k v kvs <-> lookup k kvs = Some v.
 Admitted.
+
+
+Definition inclusion_empty (A : Type) (m : list (string * A)) : inclusion [] m.
+Proof.
+  unfold inclusion. intros. inversion H.
+Qed.
+
+
 
 Lemma Lookup_functional : forall A B (k : A) (v v' : B) kvs,  Lookup k v kvs -> Lookup k v' kvs -> v = v'.
 Admitted.
@@ -61,6 +264,18 @@ Definition forall2b {A} (p : A -> A -> bool) := fix f xs ys :=
 Lemma mdrop_nil : forall X ns,
     @mdrop X ns nil = nil.
 Proof. induction ns; auto. Qed.
+
+Lemma drop_idempotent : forall X x (ns : list (string * X)), drop x (drop x ns) = drop x ns.
+Proof with auto.
+  intros.
+  induction ns...
+  - destruct a as [y v].
+    destruct (y =?x) eqn:Heqb.
+    + simpl; rewrite Heqb...
+    + repeat (simpl; rewrite Heqb).
+      congruence.
+Qed.
+
 
 Definition elem {A} (A_eqb : A -> A -> bool) (x : A) (xs : list A) :=
   match find (A_eqb x) xs with
